kk

n_mutualEx_base.thy
@@ -22,7 +22,9 @@ definition false::"scalrValueType" where [simp]: "false\<equiv> boolV False"
 
 subsection{*  Definitions of Parameterized Rules *}
 
-definition n_Try::"nat \<Rightarrow> rule" where [simp]:
+definition  NC::"nat " where [simp]: "NC==1"
+
+ definition n_Try::"nat \<Rightarrow> rule" where [simp]:
 "n_Try  i\<equiv>
 let g = (eqn (IVar (Para (Ident ''n'') i)) (Const I)) in
 let s = (parallelList [(assign ((Para (Ident ''n'') i), (Const T)))]) in
@@ -33,8 +35,6 @@ definition n_Crit::"nat \<Rightarrow> rule" where [simp]:
 let g = (andForm (eqn (IVar (Para (Ident ''n'') i)) (Const T)) (eqn (IVar (Ident ''x'')) (Const true))) in
 let s = (parallelList [(assign ((Para (Ident ''n'') i), (Const C))), (assign ((Ident ''x''), (Const false)))]) in
 guard g s"
-
-
 
 definition n_Exit::"nat \<Rightarrow> rule" where [simp]:
 "n_Exit  i\<equiv>
@@ -48,16 +48,15 @@ let g = (eqn (IVar (Para (Ident ''n'') i)) (Const E)) in
 let s = (parallelList [(assign ((Para (Ident ''n'') i), (Const I))), (assign ((Ident ''x''), (Const true)))]) in
 guard g s"
 
-definition n_Crit'::" rule" where [simp]:
-"n_Crit'  \<equiv>
-let g = ( (eqn (IVar (Ident ''x'')) (Const true))) in
-let s = (parallelList [ (assign ((Ident ''x''), (Const false)))]) in
+definition n_Crit_i_3::"rule" where [simp]:
+"n_Crit_i_3  \<equiv>
+let g = (eqn (IVar (Ident ''x'')) (Const true)) in
+let s = (parallelList [(assign ((Ident ''x''), (Const false)))]) in
 guard g s"
 
-definition n_Idle'::" nat \<Rightarrow>rule" where [simp]:
-"n_Idle' N \<equiv>
-let g = andList[(eqn (IVar (Ident ''x'')) (Const false)), 
-  forallForm (down N) (\<lambda>i. andList [neg (eqn (IVar (Para (Ident ''n'') i)) (Const E)), neg (eqn (IVar (Para (Ident ''n'') i)) (Const C))])] in
+definition n_Idle_i_3::"nat \<Rightarrow> rule" where [simp]:
+"n_Idle_i_3 N \<equiv>
+let g = (andForm (andForm (eqn (IVar (Ident ''x'')) (Const false)) (forallForm (down N) (\<lambda>j. (neg (eqn (IVar (Para (Ident ''n'') j)) (Const E)))))) (forallForm (down N) (\<lambda>j. (neg (eqn (IVar (Para (Ident ''n'') j)) (Const C)))))) in
 let s = (parallelList [(assign ((Ident ''x''), (Const true)))]) in
 guard g s"
 
@@ -67,49 +66,44 @@ definition rules::"nat \<Rightarrow> rule set" where [simp]:
 (\<exists> i. i\<le>N\<and>r=n_Try  i) \<or>
 (\<exists> i. i\<le>N\<and>r=n_Crit  i) \<or>
 (\<exists> i. i\<le>N\<and>r=n_Exit  i) \<or>
-(\<exists> i. i\<le>N\<and>r=n_Idle  i)
+(\<exists> i. i\<le>N\<and>r=n_Idle  i) \<or>
+(r=n_Crit_i_3  ) \<or>
+(r=n_Idle_i_3 N )\<or> r=skipRule
 }"
 
 
 
-definition rules'::" rule set" where [simp]:
-"rules'  \<equiv> (rules 1)  \<union> {n_Crit', n_Idle' 1}"
-
 subsection{*Definitions of a Formally Parameterized Invariant Formulas*}
 
-definition inv__1::"nat \<Rightarrow> nat \<Rightarrow> formula" where [simp]:
-"inv__1 p__Inv0 p__Inv1 \<equiv>
-(neg (andForm (eqn (IVar (Para (Ident ''n'') p__Inv0)) (Const C)) (eqn (IVar (Para (Ident ''n'') p__Inv1)) (Const C))))"
+definition inv_27::"nat \<Rightarrow> formula" where [simp]:
+"inv_27 i \<equiv>
+(implyForm (eqn (IVar (Para (Ident ''n'') i)) (Const E)) (eqn (IVar (Ident ''x'')) (Const false)))"
 
-definition inv__2::"nat \<Rightarrow> formula" where [simp]:
-"inv__2 p__Inv0 \<equiv>
-(neg (andForm (eqn (IVar (Para (Ident ''n'') p__Inv0)) (Const C)) (eqn (IVar (Ident ''x'')) (Const true))))"
+definition inv_7::"nat \<Rightarrow> nat \<Rightarrow> formula" where [simp]:
+"inv_7 i j \<equiv>
+(implyForm (eqn (IVar (Para (Ident ''n'') i)) (Const E)) (neg (eqn (IVar (Para (Ident ''n'') j)) (Const E))))"
 
-definition inv__3::"nat \<Rightarrow> nat \<Rightarrow> formula" where [simp]:
-"inv__3 p__Inv0 p__Inv1 \<equiv>
-(neg (andForm (eqn (IVar (Para (Ident ''n'') p__Inv0)) (Const C)) (eqn (IVar (Para (Ident ''n'') p__Inv1)) (Const E))))"
-
-definition inv__4::"nat \<Rightarrow> formula" where [simp]:
-"inv__4 p__Inv0 \<equiv>
-(neg (andForm (eqn (IVar (Para (Ident ''n'') p__Inv0)) (Const E)) (eqn (IVar (Ident ''x'')) (Const true))))"
-
-definition inv__5::"nat \<Rightarrow> nat \<Rightarrow> formula" where [simp]:
-"inv__5 p__Inv0 p__Inv1 \<equiv>
-(neg (andForm (eqn (IVar (Para (Ident ''n'') p__Inv0)) (Const E)) (eqn (IVar (Para (Ident ''n'') p__Inv1)) (Const E))))"
+definition inv_5::"nat \<Rightarrow> nat \<Rightarrow> formula" where [simp]:
+"inv_5 i j \<equiv>
+(implyForm (eqn (IVar (Para (Ident ''n'') i)) (Const E)) (neg (eqn (IVar (Para (Ident ''n'') j)) (Const C))))"
 
 subsection{*Definitions of  the Set of Invariant Formula Instances in a $N$-protocol Instance*}
 definition invariants::"nat \<Rightarrow> formula set" where [simp]:
 "invariants N \<equiv> {f.
-(\<exists> p__Inv0 p__Inv1. p__Inv0\<le>N\<and>p__Inv1\<le>N\<and>p__Inv0~=p__Inv1\<and>f=inv__1  p__Inv0 p__Inv1) \<or>
-(\<exists> p__Inv0. p__Inv0\<le>N\<and>f=inv__2  p__Inv0) \<or>
-(\<exists> p__Inv0 p__Inv1. p__Inv0\<le>N\<and>p__Inv1\<le>N\<and>p__Inv0~=p__Inv1\<and>f=inv__3  p__Inv0 p__Inv1) \<or>
-(\<exists> p__Inv0. p__Inv0\<le>N\<and>f=inv__4  p__Inv0) \<or>
-(\<exists> p__Inv0 p__Inv1. p__Inv0\<le>N\<and>p__Inv1\<le>N\<and>p__Inv0~=p__Inv1\<and>f=inv__5  p__Inv0 p__Inv1)
-}"
+(\<exists> i. i\<le>N\<and>f=inv_27  i) \<or>
+(\<exists> i j. i\<le>N\<and>j\<le>N\<and>i~=j\<and>f=inv_7  i j) \<or>
+(\<exists> i j. i\<le>N\<and>j\<le>N\<and>i~=j\<and>f=inv_5  i j)
+}" 
 
-
-
-subsection{*Definitions of initial states*}
+subsection{*Definitions of  the Set of Abs Invariant Formula Instances *}
+definition invariantsAbs  ::"  formula list" where [simp]:
+"invariantsAbs   \<equiv> [
+inv_27 0 ,
+inv_7 0 1 ,
+inv_7 1 0 ,
+inv_5 0 1 ,
+inv_5 1 0
+]"
 
 definition initSpec0::"nat \<Rightarrow> formula" where [simp]:
 "initSpec0 N \<equiv> (forallForm (down N) (% i . (eqn (IVar (Para (Ident ''n'') i)) (Const I))))"
@@ -122,5 +116,344 @@ definition allInitSpecs::"nat \<Rightarrow> formula list" where [simp]:
 (initSpec0 N),
 (initSpec1 )
 ]"
+axiomatization  where axiomOnf2 [simp,intro]:
+   "s ∈ reachableSet (set (allInitSpecs N )) (rules N) ⟹  1 < N ⟹ 1 < i ⟹ j<2 ⟹  formEval (f 0 1) s ⟹ formEval (f i j) s"
+
+axiomatization  where axiomOnf1 [simp,intro]:
+   "s ∈ reachableSet (set (allInitSpecs N )) (rules N) ⟹ 1 < N ⟹ 1 < i ⟹formEval (f 0 ) s ⟹ formEval (f i) s"
+
+
+
+
+subsection{*Definitions of initial states*}
+
+lemma lemmaOnn_TryGt_i:
+  assumes a1:"i>NC" and a2:"s ∈ reachableSet (set (allInitSpecs N)) (rules N)"  and  
+  a4:"∀f.  f ∈(set invariantsAbs) ⟶  formEval f s" 
+shows "trans_sim_on1 (n_Try i  ) skipRule (set invariantsAbs) s" (is "trans_sim_on1 ?r ?r' ?F s")
+proof(unfold trans_sim_on1_def,(rule allI)+,(rule impI)+,rule disjI2)
+  fix s2 
+  assume b0:"state_sim_on1 s s2 (set invariantsAbs)"
+  show "state_sim_on1 (trans (act (n_Try i)) s) s2 (set invariantsAbs)"
+  proof(cut_tac a1,unfold state_sim_on1_def,
+    (rule allI)+,(rule impI)+)
+    fix f v
+    assume b1:" f ∈(set invariantsAbs)" and b2:"v ∈ varOfForm f"  
+
+    have b30: "(varOfFormList  invariantsAbs) = {v. ∃f. f ∈ set  invariantsAbs∧ v ∈ varOfForm f}"
+      using setOfList by blast
+      
+     
+    from b1 and b2 and b30 have b4:"v ∈ (varOfFormList  invariantsAbs)" by blast
+     
+    from b4 have b5:"trans (act (n_Try  i)) s v = s v" 
+      by (cut_tac a1  b4  ,auto) 
+
+    from b0   have b6:"s v =s2 v "
+      using b1 b2 state_sim_on1_def by blast  
+    show "trans (act (n_Try i)) s v= s2 v"
+      using b5 b6 by auto 
+  qed
+qed
+lemma lemmaOnn_TryLeNc_:
+  assumes a1:"i\<le>NC" 
+  shows "trans_sim_on1 (n_Try i) (n_Try i) (set invariantsAbs) s" (is "trans_sim_on1 ?r ?r ?F s")
+proof(rule ruleSimId)
+  show  "∀v. v∈varOfForm (pre ?r) ⟶  v ∈(varOfFormList invariantsAbs) "
+    by(cut_tac a1, auto) 
+    
+next
+  show  b1: "∀v a. a ∈ set (statement2Assigns (act ?r)) ⟶ v∈varOfExp ( substExpByStatement (IVar (fst a))  (act ?r))⟶v ∈varOfFormList invariantsAbs "
+   proof(cut_tac a1,(rule allI)+,(rule impI)+,auto) qed
+    
+ qed
+lemma lemmaOnn_Try: 
+  assumes   a2:"s ∈ reachableSet (set (allInitSpecs N)) (rules N)"  and  
+  a4:"∀f.  f ∈(set invariantsAbs) ⟶  formEval f s" and a5:"\<exists> i. i\<le>N\<and>r=n_Try  i"
+  shows "∃ r'. r' ∈ rules NC∧ trans_sim_on1 r r' (set invariantsAbs) s" (is "∃r'.?P1 r' ∧ ?P2 r'")
+proof -
+  from a5 obtain i where d0:"i\<le>N\<and>r=n_Try  i"  by blast
+  have "i>NC|i\<le> NC" by auto
+  moreover{
+       assume a1:"i>NC" 
+        have "∃r'. ?P1 r' ∧ ?P2 r'"
+        proof(rule_tac x="(skipRule)" in exI,rule conjI)
+          show  "?P1 (skipRule) " 
+           by(cut_tac a1, auto) 
+          next
+          show  "?P2 (skipRule) "
+           using lemmaOnn_TryGt_i local.a1 a2 a4 d0 by blast 
+        qed
+       }
+moreover{
+       assume a1:"i\<le> NC" 
+        have "∃r'. ?P1 r' ∧ ?P2 r'"
+        proof(rule_tac x="(n_Try i)" in exI,rule conjI)
+          show  "?P1 (n_Try i) " 
+           by(cut_tac a1, auto) 
+          next
+          show  "?P2 (n_Try i) "
+           using lemmaOnn_TryLeNc_ local.a1 a2 a4 d0 by blast 
+        qed
+       }
+  ultimately show "∃r'.?P1 r' ∧ ?P2 r'" 
+    by satx
+qed
+
+lemma lemmaOnn_CritGt_i:
+  assumes a1:"i>NC" and 
+  a2:"s ∈ reachableSet (set (allInitSpecs N)) (rules N)"  and a3:"NC<N" and  
+  a4:"∀f.  f ∈(set invariantsAbs) ⟶  formEval f s" 
+  shows "trans_sim_on1 (n_Crit i)  (n_Crit_i_3  ) (set invariantsAbs) s" (is "trans_sim_on1 ?r ?r' (set ?F) s")  (*why (n_Crit_i_3*)
+  proof(rule ruleSimCond1)
+    show " formEval (pre ?r) s ⟶formEval (pre ?r') s" (is "?A ⟶?B")
+    proof(rule impI)+
+      assume b0:"?A"
+  
+      from b0  show "formEval (pre ?r') s" 
+       by auto
+     qed
+   next 
+	show "(∀  v. v ∈  varOfSent (act  ?r') ⟶  v ∈ varOfFormList ?F ⟶ formEval (pre ?r) s ⟶ 
+    expEval (substExpByStatement (IVar v)  (act ?r')) s = expEval (substExpByStatement (IVar v)  (act ?r)) s)"
+   proof(rule allI,(rule impI)+)
+      fix  v
+     assume b1:"v∈ (varOfFormList invariantsAbs)"  and b2:"formEval (pre ?r) s" and b3:"v ∈varOfSent (act ?r')"
+  
+  show "expEval (substExpByStatement (IVar v)  (act ?r')) s = expEval (substExpByStatement (IVar v)  (act ?r)) s"  
+       apply (cut_tac  a1 b1 b2 ,auto) done
+   qed
+ next
+   show "∀  v. v ∈  varOfSent (act ?r) ⟶  v ∈ varOfFormList ?F ⟶ v ∈  varOfSent (act ?r')" by(cut_tac a1, auto)
+
+  
+ next 
+   show "∀ v va. v ∈ varOfSent (act ?r') ⟶va∈varOfExp ( substExpByStatement (IVar v)  (act ?r'))⟶ va ∈ (varOfFormList ?F)"
+     by auto  
+ next
+   show "∀v. v ∈ varOfForm (pre (?r')) ⟶ v ∈ varOfFormList ?F" by auto
+qed
+lemma lemmaOnn_CritLeNc_:
+  assumes a1:"i\<le>NC" 
+  shows "trans_sim_on1 (n_Crit i) (n_Crit i) (set invariantsAbs) s" (is "trans_sim_on1 ?r ?r ?F s")
+proof(rule ruleSimId)
+  show  "∀v. v∈varOfForm (pre ?r) ⟶  v ∈(varOfFormList invariantsAbs) "
+    by(cut_tac a1, auto) 
+    
+next
+  show  b1: "∀v a. a ∈ set (statement2Assigns (act ?r)) ⟶ v∈varOfExp ( substExpByStatement (IVar (fst a))  (act ?r))⟶v ∈varOfFormList invariantsAbs "
+   proof(cut_tac a1,(rule allI)+,(rule impI)+,auto) qed
+    
+ qed
+lemma lemmaOnn_Crit: 
+  assumes   a2:"s ∈ reachableSet (set (allInitSpecs N)) (rules N)"  and  
+  a4:"∀f.  f ∈(set invariantsAbs) ⟶  formEval f s" and a5:"\<exists> i. i\<le>N\<and>r=n_Crit  i"
+  and a6:"NC <N"
+  shows "∃ r'. r' ∈ rules NC∧ trans_sim_on1 r r' (set invariantsAbs) s" (is "∃r'.?P1 r' ∧ ?P2 r'")
+proof -
+  from a5 obtain i where d0:"i\<le>N\<and>r=n_Crit  i"  by blast
+  have "i>NC|i\<le> NC" by auto
+  moreover{
+       assume a1:"i>NC" 
+        have "∃r'. ?P1 r' ∧ ?P2 r'"
+        proof(rule_tac x="(n_Crit_i_3)" in exI,rule conjI)
+          show  "?P1 (n_Crit_i_3) " 
+           by(cut_tac a1, auto) 
+          next
+          show  "?P2 (n_Crit_i_3) "
+           using lemmaOnn_CritGt_i local.a1 a2 a4 a6 d0 by blast 
+        qed
+       }
+moreover{
+       assume a1:"i\<le> NC" 
+        have "∃r'. ?P1 r' ∧ ?P2 r'"
+        proof(rule_tac x="(n_Crit i)" in exI,rule conjI)
+          show  "?P1 (n_Crit i) " 
+           by(cut_tac a1, auto) 
+          next
+          show  "?P2 (n_Crit i) "
+           using lemmaOnn_CritLeNc_ local.a1 a2 a4 d0 by blast 
+        qed
+       }
+  ultimately show "∃r'.?P1 r' ∧ ?P2 r'" 
+    by satx
+qed
+
+lemma lemmaOnn_ExitGt_i:
+  assumes a1:"i>NC" and a2:"s ∈ reachableSet (set (allInitSpecs N)) (rules N)"  and  
+  a4:"∀f.  f ∈(set invariantsAbs) ⟶  formEval f s" 
+shows "trans_sim_on1 (n_Exit i  ) skipRule (set invariantsAbs) s" (is "trans_sim_on1 ?r ?r' ?F s")
+proof(unfold trans_sim_on1_def,(rule allI)+,(rule impI)+,rule disjI2)
+  fix s2 
+  assume b0:"state_sim_on1 s s2 (set invariantsAbs)"
+  show "state_sim_on1 (trans (act (n_Try i)) s) s2 (set invariantsAbs)"
+  proof(cut_tac a1,unfold state_sim_on1_def,
+    (rule allI)+,(rule impI)+)
+    fix f v
+    assume b1:" f ∈(set invariantsAbs)" and b2:"v ∈ varOfForm f"  
+
+    have b30: "(varOfFormList  invariantsAbs) = {v. ∃f. f ∈ set  invariantsAbs∧ v ∈ varOfForm f}"
+      using setOfList by blast
+      
+     
+    from b1 and b2 and b30 have b4:"v ∈ (varOfFormList  invariantsAbs)" by blast
+     
+    from b4 have b5:"trans (act (n_Try  i)) s v = s v" 
+      by (cut_tac a1  b4  ,auto) 
+
+    from b0   have b6:"s v =s2 v "
+      using b1 b2 state_sim_on1_def by blast  
+    show "trans (act (n_Try i)) s v= s2 v"
+      using b5 b6 by auto 
+  qed
+qed
+lemma lemmaOnn_ExitLeNc_:
+  assumes a1:"i\<le>NC" 
+  shows "trans_sim_on1 (n_Exit i) (n_Exit i) (set invariantsAbs) s" (is "trans_sim_on1 ?r ?r ?F s")
+proof(rule ruleSimId)
+  show  "∀v. v∈varOfForm (pre ?r) ⟶  v ∈(varOfFormList invariantsAbs) "
+    by(cut_tac a1, auto) 
+    
+next
+  show  b1: "∀v a. a ∈ set (statement2Assigns (act ?r)) ⟶ v∈varOfExp ( substExpByStatement (IVar (fst a))  (act ?r))⟶v ∈varOfFormList invariantsAbs "
+   proof(cut_tac a1,(rule allI)+,(rule impI)+,auto) qed
+    
+ qed
+lemma lemmaOnn_Exit: 
+  assumes   a2:"s ∈ reachableSet (set (allInitSpecs N)) (rules N)"  and  
+  a4:"∀f.  f ∈(set invariantsAbs) ⟶  formEval f s" and a5:"\<exists> i. i\<le>N\<and>r=n_Exit  i"
+  shows "∃ r'. r' ∈ rules NC∧ trans_sim_on1 r r' (set invariantsAbs) s" (is "∃r'.?P1 r' ∧ ?P2 r'")
+proof -
+  from a5 obtain i where d0:"i\<le>N\<and>r=n_Exit  i"  by blast
+  have "i>NC|i\<le> NC" by auto
+  moreover{
+       assume a1:"i>NC" 
+        have "∃r'. ?P1 r' ∧ ?P2 r'"
+        proof(rule_tac x="(skipRule)" in exI,rule conjI)
+          show  "?P1 (skipRule) " 
+           by(cut_tac a1, auto) 
+          next
+          show  "?P2 (skipRule) "
+           using lemmaOnn_ExitGt_i local.a1 a2 a4 d0 by blast 
+        qed
+       }
+moreover{
+       assume a1:"i\<le> NC" 
+        have "∃r'. ?P1 r' ∧ ?P2 r'"
+        proof(rule_tac x="(n_Exit i)" in exI,rule conjI)
+          show  "?P1 (n_Exit i) " 
+           by(cut_tac a1, auto) 
+          next
+          show  "?P2 (n_Exit i) "
+           using lemmaOnn_ExitLeNc_ local.a1 a2 a4 d0 by blast 
+        qed
+       }
+  ultimately show "∃r'.?P1 r' ∧ ?P2 r'" 
+    by satx
+qed
+
+lemma lemmaOnn_IdleGt_i:
+  assumes a1:"i>NC" and 
+  a2:"s ∈ reachableSet (set (allInitSpecs N)) (rules N)"  and a3:"NC<N" and  
+  a4:"∀f.  f ∈(set invariantsAbs) ⟶  formEval f s" 
+  shows "trans_sim_on1 (n_Idle i)  (n_Idle_i_3  NC) (set invariantsAbs) s" (is "trans_sim_on1 ?r ?r' (set ?F) s")
+  proof(rule ruleSimCond1)
+    show " formEval (pre ?r) s ⟶formEval (pre ?r') s" (is "?A ⟶?B")
+    proof(rule impI)+
+      assume b0:"?A"
+  from a4  have tmp:"formEval (inv_27 0)  s"   
+            by (force simp del:inv_27_def) 
+        have tmp1:"formEval (inv_27 i  ) s" 
+        proof(cut_tac a1 a2 a3 tmp,rule axiomOnf1,force+)qed
+        with b0  have c0:"formEval  (conclude (inv_27 i)) s" by auto
+from a4  have tmp:"formEval (inv_7 0 1)  s"   
+            by (force simp del:inv_7_def) 
+        have tmp1:"formEval (inv_7 i 0  ) s" 
+        proof(cut_tac a1 a2 a3 tmp,rule axiomOnf2,force+)qed
+        with b0  have c1:"formEval  (conclude (inv_7 i 0)) s" by auto
+from a4  have tmp:"formEval (inv_7 0 1)  s"   
+            by (force simp del:inv_7_def) 
+        have tmp1:"formEval (inv_7 i 1  ) s" 
+        proof(cut_tac a1 a2 a3 tmp,rule axiomOnf2,force+)qed
+        with b0  have c2:"formEval  (conclude (inv_7 i 1)) s" by auto
+from a4  have tmp:"formEval (inv_5 0 1)  s"   
+            by (force simp del:inv_5_def) 
+        have tmp1:"formEval (inv_5 i 0  ) s" 
+        proof(cut_tac a1 a2 a3 tmp,rule axiomOnf2,force+)qed
+        with b0  have c3:"formEval  (conclude (inv_5 i 0)) s" by auto
+from a4  have tmp:"formEval (inv_5 0 1)  s"   
+            by (force simp del:inv_5_def) 
+        have tmp1:"formEval (inv_5 i 1  ) s" 
+        proof(cut_tac a1 a2 a3 tmp,rule axiomOnf2,force+)qed
+        with b0  have c4:"formEval  (conclude (inv_5 i 1)) s" by auto
+
+      from b0 c0 c1 c2 c3 c4 show "formEval (pre ?r') s" 
+       by auto
+     qed
+   next 
+	show "(∀  v. v ∈  varOfSent (act  ?r') ⟶  v ∈ varOfFormList ?F ⟶ formEval (pre ?r) s ⟶ 
+    expEval (substExpByStatement (IVar v)  (act ?r')) s = expEval (substExpByStatement (IVar v)  (act ?r)) s)"
+   proof(rule allI,(rule impI)+)
+      fix  v
+     assume b1:"v∈ (varOfFormList invariantsAbs)"  and b2:"formEval (pre ?r) s" and b3:"v ∈varOfSent (act ?r')"
+  
+  show "expEval (substExpByStatement (IVar v)  (act ?r')) s = expEval (substExpByStatement (IVar v)  (act ?r)) s"  
+       apply (cut_tac  a1 b1 b2 ,auto) done
+   qed
+ next
+   show "∀  v. v ∈  varOfSent (act ?r) ⟶  v ∈ varOfFormList ?F ⟶ v ∈  varOfSent (act ?r')" by(cut_tac a1, auto)
+
+  
+ next 
+   show "∀ v va. v ∈ varOfSent (act ?r') ⟶va∈varOfExp ( substExpByStatement (IVar v)  (act ?r'))⟶ va ∈ (varOfFormList ?F)"
+     by auto  
+ next
+   show "∀v. v ∈ varOfForm (pre (?r')) ⟶ v ∈ varOfFormList ?F" by auto
+qed
+lemma lemmaOnn_IdleLeNc_:
+  assumes a1:"i\<le>NC" 
+  shows "trans_sim_on1 (n_Idle i) (n_Idle i) (set invariantsAbs) s" (is "trans_sim_on1 ?r ?r ?F s")
+proof(rule ruleSimId)
+  show  "∀v. v∈varOfForm (pre ?r) ⟶  v ∈(varOfFormList invariantsAbs) "
+    by(cut_tac a1, auto) 
+    
+next
+  show  b1: "∀v a. a ∈ set (statement2Assigns (act ?r)) ⟶ v∈varOfExp ( substExpByStatement (IVar (fst a))  (act ?r))⟶v ∈varOfFormList invariantsAbs "
+   proof(cut_tac a1,(rule allI)+,(rule impI)+,auto) qed
+    
+ qed
+lemma lemmaOnn_Idle: 
+  assumes   a2:"s ∈ reachableSet (set (allInitSpecs N)) (rules N)"  and  
+  a4:"∀f.  f ∈(set invariantsAbs) ⟶  formEval f s" and a5:"\<exists> i. i\<le>N\<and>r=n_Idle  i"
+  shows "∃ r'. r' ∈ rules NC∧ trans_sim_on1 r r' (set invariantsAbs) s" (is "∃r'.?P1 r' ∧ ?P2 r'")
+proof -
+  from a5 obtain i where d0:"i\<le>N\<and>r=n_Idle  i"  by blast
+  have "i>NC|i\<le> NC" by auto
+  moreover{
+       assume a1:"i>NC" 
+        have "∃r'. ?P1 r' ∧ ?P2 r'"
+        proof(rule_tac x="(n_Idle  NC)" in exI,rule conjI)
+          show  "?P1 (n_Idle  NC) " 
+           by(cut_tac a1, auto) 
+          next
+          show  "?P2 (n_Idle  NC) "
+           using lemmaOnn_IdleGt_i local.a1 a2 a4 d0 by blast 
+        qed
+       }
+moreover{
+       assume a1:"i\<le> NC" 
+        have "∃r'. ?P1 r' ∧ ?P2 r'"
+        proof(rule_tac x="(n_Idle i)" in exI,rule conjI)
+          show  "?P1 (n_Idle i) " 
+           by(cut_tac a1, auto) 
+          next
+          show  "?P2 (n_Idle i) "
+           using lemmaOnn_IdleLeNc_ local.a1 a2 a4 d0 by blast 
+        qed
+       }
+  ultimately show "∃r'.?P1 r' ∧ ?P2 r'" 
+    by satx
+qed
+
 
 end
